More work on polymorphic expressions

theories/core/utp_poly_expr.thy
@@ -35,32 +35,119 @@ lemma Rep_WF_PEXPRESSION_elim [elim]:
 
 setup_lifting type_definition_WF_PEXPRESSION
 
-notation Rep_WF_PEXPRESSION ("\<langle>_\<rangle>\<^sub>~")
+notation Rep_WF_PEXPRESSION ("\<langle>_\<rangle>\<^sub>*")
 
 lemma Rep_WF_EXPRESSION_typed [typing]:
-  "\<langle>e\<rangle>\<^sub>~ t :\<^sub>e t"
+  "\<langle>e\<rangle>\<^sub>* t :\<^sub>e t"
   apply (insert Rep_WF_PEXPRESSION[of e])
   apply (auto simp add:WF_PEXPRESSION_def)
 done
 
-definition CoercePE :: "'a WF_PEXPRESSION \<Rightarrow> 'a UTYPE \<Rightarrow> 'a WF_EXPRESSION" where
-"CoercePE e t = \<langle>e\<rangle>\<^sub>~ t"
+subsection {* Core syntax *}
+
+default_sort BOT_SORT
+
+definition monopexpr :: "'a WF_PEXPRESSION \<Rightarrow> bool" where
+"monopexpr e = (\<exists>! t. \<D> (\<langle>e\<rangle>\<^sub>* t))"
+
+definition petype_rel :: "'a WF_PEXPRESSION \<Rightarrow> 'a UTYPE \<Rightarrow> bool" (infix ":\<^sub>*" 50) where
+"petype_rel e t \<equiv> \<D> (\<langle>e\<rangle>\<^sub>* t)"
+
+definition pexpr_type :: "'a WF_PEXPRESSION \<Rightarrow> 'a UTYPE" ("\<tau>\<^sub>*") where
+"pexpr_type e = (THE t. \<D> (\<langle>e\<rangle>\<^sub>* t))"
+
+lift_definition CoercePE :: "'a WF_PEXPRESSION \<Rightarrow> 'a UTYPE \<Rightarrow> 'a WF_PEXPRESSION" is
+"\<lambda> e t t'. (if (t = t') then \<langle>e\<rangle>\<^sub>* t else BotE t')"
+  by (auto intro:typing simp add:WF_PEXPRESSION_def)
+
+(* Convert to an fully disambiguated polymorphic expression to a basic expression *)
+definition PExprE :: "'a WF_PEXPRESSION \<Rightarrow> 'a WF_EXPRESSION" where
+"PExprE e = \<langle>e\<rangle>\<^sub>* (pexpr_type e)"
+
+lift_definition LitPE :: "'a::BOT_SORT \<Rightarrow> 'a WF_PEXPRESSION" is
+"\<lambda> v t. if (v : t) then LitE v else BotE t"
+  by (auto simp add:WF_PEXPRESSION_def typing)
+
+subsubsection {* Laws *}
+
+lemma LitPE_type [typing]:
+  "v :! t \<Longrightarrow> LitPE v :\<^sub>* t"
+  by (simp add: petype_rel_def LitPE.rep_eq defined typing)
+
+lemma LitPE_monopexpr [closure]:
+  "\<lbrakk> v :! t; monotype t \<rbrakk> \<Longrightarrow> monopexpr (LitPE v)"
+  apply (simp add:monopexpr_def LitPE.rep_eq defined monotype_def)
+  apply (rule_tac a="t" in ex1I)
+  apply (auto simp add:dtype_rel_def)
+done
+
+lemma CoercePE_monopexpr [closure]: 
+  "\<D> (\<langle>e\<rangle>\<^sub>* t) \<Longrightarrow> monopexpr (CoercePE e t)"
+  apply (simp add: monopexpr_def CoercePE.rep_eq)
+  apply (rule_tac a="t" in ex1I)
+  apply (auto simp add:defined)
+done
+
+lemma monopexpr_tau [simp]: "\<lbrakk> x :\<^sub>* t; monopexpr x \<rbrakk> \<Longrightarrow> \<tau>\<^sub>* x = t"
+  apply (simp add: petype_rel_def pexpr_type_def monotype_def monopexpr_def)
+  apply (rule the_equality)
+  apply (auto)
+done
+
+subsection {* Boolean Expressions *}
+
+abbreviation "TruePE \<equiv> LitPE (MkBool True)"
+abbreviation "FalsePE \<equiv> LitPE (MkBool False)"
+
+subsubsection {* Laws *}
+
+lemma TruePE_monopexpr [closure]:
+  "monopexpr TruePE"
+  by (auto intro:closure typing)
+
+lemma FalsePE_monopexpr [closure]:
+  "monopexpr FalsePE"
+  by (auto intro:closure typing)
 
 subsection {* List Expressions *}
 
-lift_definition NilPE :: "'a::{BOT_SORT, LIST_SORT} WF_PEXPRESSION" 
+default_sort "{BOT_SORT, LIST_SORT}"
+
+lift_definition NilPE :: "'a WF_PEXPRESSION" 
 is "\<lambda> a. if (isListType a \<and> ListParam a \<in> ListPerm) 
          then NilE (ListParam a) else BotE a"
   by (force intro:typing simp add:WF_PEXPRESSION_def)
 
 lift_definition ConsPE :: 
-  "'a::{BOT_SORT, LIST_SORT} WF_PEXPRESSION \<Rightarrow> 'a WF_PEXPRESSION \<Rightarrow> 'a WF_PEXPRESSION" 
+  "'a WF_PEXPRESSION \<Rightarrow> 'a WF_PEXPRESSION \<Rightarrow> 'a WF_PEXPRESSION" 
 is "\<lambda> x xs a. if (isListType a \<and> ListParam a \<in> ListPerm \<and> \<D> (x (ListParam a)) \<and> \<D> (xs a))
               then ConsE (ListParam a) (x (ListParam a)) (xs a) else BotE a"
   by (force intro:typing simp add:WF_PEXPRESSION_def)
 
-(* Convert to an fully disambiguated polymorphic expression to a basic expression *)
-definition PExprE :: "'a WF_PEXPRESSION \<Rightarrow> 'a WF_EXPRESSION" where
-"PExprE e = \<langle>e\<rangle>\<^sub>~ (THE t. \<D> (\<langle>e\<rangle>\<^sub>~ t))"
+lift_definition ConcatPE ::
+  "'a WF_PEXPRESSION \<Rightarrow> 'a WF_PEXPRESSION \<Rightarrow> 'a WF_PEXPRESSION"
+is "\<lambda> xs ys a. if (isListType a \<and> ListParam a \<in> ListPerm \<and> \<D> (xs a) \<and> \<D> (ys a))
+               then ConcatE (ListParam a) (xs a) (ys a) else BotE a"
+  by (force intro:typing simp add:WF_PEXPRESSION_def)
+
+lemma NilPE_type [typing]: "a \<in> ListPerm \<Longrightarrow> NilPE :\<^sub>* ListType a"
+  by (simp add:petype_rel_def NilPE.rep_eq typing defined)
+
+lemma ConsPE_type [typing]: 
+  "\<lbrakk> a \<in> ListPerm; x :\<^sub>* a; xs :\<^sub>* ListType a \<rbrakk> \<Longrightarrow> ConsPE x xs :\<^sub>* ListType a"
+  by (force intro:typing defined simp add:petype_rel_def ConsPE.rep_eq typing defined)
+
+lemma ConcatPE_type [typing]: 
+  "\<lbrakk> a \<in> ListPerm; xs :\<^sub>* ListType a; ys :\<^sub>* ListType a \<rbrakk> 
+   \<Longrightarrow> ConcatPE xs ys :\<^sub>* ListType a"
+  by (force intro:typing defined simp add:petype_rel_def ConcatPE.rep_eq typing defined)
+
+lemma ConsE_monopexpr [typing]:
+  "\<lbrakk> monopexpr x; x :\<^sub>* t; xs :\<^sub>* ListType t; t \<in> ListPerm \<rbrakk> \<Longrightarrow> monopexpr (ConsPE x xs)"
+  apply (simp add:monopexpr_def ConsPE.rep_eq defined typing petype_rel_def)
+  apply (rule_tac a="ListType t" in ex1I)
+  apply (auto intro:typing defined)
+  apply (metis ListParam isListType_elim)
+done
 
 end
